cedar-lean/Cedar/Thm/Partial/Evaluation/Record.lean
@@ -1,0 +1,226 @@
+/-
+ Copyright 2022-2023 Amazon.com, Inc. or its affiliates. All Rights Reserved.
+
+ Licensed under the Apache License, Version 2.0 (the "License");
+ you may not use this file except in compliance with the License.
+ You may obtain a copy of the License at
+
+      https://www.apache.org/licenses/LICENSE-2.0
+
+ Unless required by applicable law or agreed to in writing, software
+ distributed under the License is distributed on an "AS IS" BASIS,
+ WITHOUT WARRANTIES OR CONDITIONS OF ANY KIND, either express or implied.
+ See the License for the specific language governing permissions and
+ limitations under the License.
+-/
+
+import Cedar.Partial.Evaluator
+import Cedar.Spec.Policy
+import Cedar.Thm.Data.Control
+import Cedar.Thm.Partial.Evaluation.Basic
+import Cedar.Thm.Utils
+
+namespace Cedar.Thm.Partial.Evaluation.Record
+
+open Cedar.Data
+open Cedar.Spec (Attr Error Result)
+open Except
+
+/--
+  helper lemma: any subexpression of x is a subexpression of any record containing x
+-/
+theorem value_subexpression {x₁ x₂ : Partial.Expr} {attrs : List (Attr × Partial.Expr)} :
+  x₁ ∈ attrs.map Prod.snd → x₂ ∈ x₁.subexpressions → x₂ ∈ (Partial.Expr.record attrs).subexpressions
+:= by
+  intro h₁ h₂
+  unfold Partial.Expr.subexpressions
+  simp [List.append_eq_append]
+  right
+  have h₃ := List.mem_map_of_mem Partial.Expr.subexpressions h₁
+  rw [List.map_map] at h₃
+  apply List.mem_join_of_mem h₃ h₂
+
+/--
+  helper lemma: if any component of a `record` contains an unknown, the whole
+  expression does
+-/
+theorem value_unknown {x : Partial.Expr} {attrs : List (Attr × Partial.Expr)} :
+  x ∈ attrs.map Prod.snd → x.containsUnknown → (Partial.Expr.record attrs).containsUnknown
+:= by
+  unfold Partial.Expr.containsUnknown
+  repeat rw [List.any_eq_true]
+  intro h₁ h₂
+  replace ⟨subx, h₂⟩ := h₂
+  exists subx
+  constructor
+  case left => apply value_subexpression h₁ h₂.left
+  case right => exact h₂.right
+
+/--
+  `Partial.bindAttr` on concrete arguments is the same as `Spec.bindAttr` on
+  those arguments
+-/
+theorem Partial.bindAttr_on_concrete_eqv_bindAttr {a : Attr} {res : Result Spec.Value} :
+  Partial.bindAttr a (res.map Partial.Value.value) = (Spec.bindAttr a res).map λ (k, v) => (k, Partial.Value.value v)
+:= by
+  unfold Partial.bindAttr Spec.bindAttr
+  cases res <;> simp [Except.map]
+
+/--
+  `List.mapM_pmap_subtype` specialized for a particular setting involving pairs
+-/
+theorem mapM_pmap_subtype_snd
+  {p : (Attr × β) → Prop}
+  (f : β → Result Spec.Value)
+  (pairs: List (Attr × β))
+  (h : ∀ pair ∈ pairs, p pair) :
+  List.mapM (λ x : {pair : (Attr × β) // p pair} => Spec.bindAttr x.val.fst (f x.val.snd)) (List.pmap Subtype.mk pairs h) =
+  pairs.mapM (λ x => Spec.bindAttr x.fst (f x.snd))
+:= by
+  rw [←List.mapM'_eq_mapM]
+  induction pairs <;> simp [*]
+
+/--
+  `List.mapM_pmap_subtype` specialized for a particular setting involving pairs
+-/
+theorem mapM_pmap_subtype_snd'
+  {p : (Attr × β) → Prop}
+  (f : β → Result Partial.Value)
+  (pairs: List (Attr × β))
+  (h : ∀ pair ∈ pairs, p pair) :
+  List.mapM (λ x : {pair : (Attr × β) // p pair} => Partial.bindAttr x.val.fst (f x.val.snd)) (List.pmap Subtype.mk pairs h) =
+  pairs.mapM (λ x => Partial.bindAttr x.fst (f x.snd))
+:= by
+  rw [←List.mapM'_eq_mapM]
+  induction pairs <;> simp [*]
+
+/--
+  `List.mapM₂_eq_mapM` specialized for a particular setting involving pairs
+-/
+theorem mapM₂_eq_mapM_specialized [SizeOf β]
+  (f : β → Result Spec.Value)
+  (attrs : List (Attr × β)) :
+  attrs.mapM₂
+    (λ x : {x : Attr × β // sizeOf x.snd < 1 + sizeOf attrs} => match x with
+      | ⟨(a, b), _⟩ => Spec.bindAttr a (f b)
+    ) =
+  attrs.mapM λ (a, b) => Spec.bindAttr a (f b)
+:= by
+  simp [List.mapM₂, List.attach₂, mapM_pmap_subtype_snd]
+
+/--
+  `List.mapM₂_eq_mapM` specialized for a particular setting involving pairs
+-/
+theorem mapM₂_eq_mapM_specialized' [SizeOf β]
+  (f : β → Result Partial.Value)
+  (attrs : List (Attr × β)) :
+  attrs.mapM₂
+    (λ x : {x : Attr × β // sizeOf x.snd < 1 + sizeOf attrs} => match x with
+      | ⟨(a, b), _⟩ => Partial.bindAttr a (f b)
+    ) =
+  attrs.mapM λ (a, b) => Partial.bindAttr a (f b)
+:= by
+  simp [List.mapM₂, List.attach₂, mapM_pmap_subtype_snd']
+
+/--
+  Inductive argument that partial evaluating a concrete `Partial.Expr.record`
+  expression gives the same output as concrete-evaluating the `Spec.Expr.record`
+  with the same subexpressions
+-/
+theorem partial_eval_on_concrete_eqv_concrete_eval {attrs : List (Attr × Spec.Expr)} {request : Spec.Request} {entities : Spec.Entities} :
+  (∀ kv ∈ attrs, Partial.evaluate kv.snd request entities = (Spec.evaluate kv.snd request entities).map Partial.Value.value) →
+  Partial.evaluate (Partial.Expr.record (attrs.map₁ λ ⟨(k, v), _⟩ => (k, v.asPartialExpr))) request entities = (Spec.evaluate (Spec.Expr.record attrs) request entities).map Partial.Value.value
+:= by
+  intro ih₁
+  unfold Partial.evaluate Spec.evaluate
+  rw [List.map₁_eq_map_snd Spec.Expr.asPartialExpr attrs]
+  rw [mapM₂_eq_mapM_specialized (Spec.evaluate · request entities) attrs]
+  rw [mapM₂_eq_mapM_specialized' (Partial.evaluate · request entities) _]
+  induction attrs
+  case nil => simp [Except.map, pure, Except.pure]
+  case cons kv attrs' h_ind =>
+    specialize h_ind (by
+      intro kv' h₁
+      apply ih₁ kv' (List.mem_cons_of_mem kv h₁)
+    )
+    cases h₁ : Spec.bindAttr kv.fst (Spec.evaluate kv.snd request entities)
+    <;> cases h₂ : Partial.bindAttr kv.fst (Partial.evaluate kv.snd request entities)
+    <;> cases h₃ : Spec.evaluate kv.snd request entities
+    <;> simp [h₁, h₂]
+    <;> simp [ih₁ kv, Except.map, pure, Except.pure] at h₂
+    <;> simp [h₃, Spec.bindAttr, Partial.bindAttr] at h₁ h₂
+    case error.error.error e₁ e₂ e₃ =>
+      simp [Except.map, pure, Except.pure]
+      subst h₁ h₂
+      rfl
+    case ok.ok.ok val' pval val =>
+      subst h₁ h₂
+      simp [List.mapM_map]
+      simp [List.mapM_map] at h_ind
+      -- the remaning goal is just a statement about `attrs'`, not `kv` itself
+      -- so we can dispatch it using `h_ind`
+      generalize h₃ : (attrs'.mapM λ x => Partial.bindAttr x.fst (Partial.evaluate x.snd.asPartialExpr request entities)) = pres at *
+      generalize h₄ : (attrs'.mapM λ x => Spec.bindAttr x.fst (Spec.evaluate x.snd request entities)) = sres at *
+      cases pres <;> cases sres <;> simp [Except.map, pure, Except.pure] at *
+      case error.error e₁ e₂ => exact h_ind
+      case ok.error pvals e =>
+        -- here, partial evaluation of `attrs'` produced `ok` (h₃), while concrete
+        -- evaluation of `attrs'` produced `error` (h₄).
+        -- this contradicts `h_ind`.
+        exfalso
+        split at h_ind <;> simp at h_ind
+      case ok.ok pvals vals =>
+        -- here, partial evaluation of `xs'` produced `ok pvals` (h₃), while
+        -- concrete evaluation of `xs'` produced `ok vals` (h₄), and we need to
+        -- show a particular relationship between `pvals` and `vals` using `h_ind`.
+        split at h_ind <;> simp at h_ind
+        case h_1 vals' h₂ =>
+          simp [h₂]
+          exact Map.make_cons h_ind
+
+/--
+  Inductive argument for `ResidualsContainUnknowns` for `Partial.Expr.set`
+-/
+theorem residuals_contain_unknowns {attrs : List (Attr × Partial.Expr)} {request : Partial.Request} {entities : Partial.Entities} :
+  (∀ kv ∈ attrs, @Partial.Expr.ResidualsContainUnknowns kv.snd request entities) →
+  @Partial.Expr.ResidualsContainUnknowns (Partial.Expr.record attrs) request entities
+:= by
+  unfold Partial.Expr.ResidualsContainUnknowns
+  intro ih₁ r h₁
+  -- the entire record evaluated to `.residual r`. we must show that `r` contains
+  -- an unknown
+  unfold Partial.evaluate at h₁
+  rw [mapM₂_eq_mapM_specialized' (Partial.evaluate · request entities) attrs] at h₁
+  cases h₂ : (attrs.mapM λ x => match x with | (k, v) => Partial.bindAttr k (Partial.evaluate v request entities))
+  <;> simp [h₂] at h₁
+  case ok pvals =>
+    split at h₁ <;> simp at h₁
+    -- naturally, the residual `r` which the record evaluated to, is itself a `.record`
+    -- with elements `pvals.map Partial.Value.asPartialExpr`
+    all_goals subst h₁
+    -- so now we have to show that `(.record (pvals.map Partial.Value.asPartialExpr))`
+    -- contains an unknown
+    case h_2 h₃ =>
+      -- in this case, some element of the record evaluated to a residual
+      rw [mapM_none_iff_f_none_on_some_element] at h₃
+      replace ⟨(a, pval), h₃, h₄⟩ := h₃
+      split at h₄ <;> simp at h₄
+      case h_2 r h₅ =>
+        -- `.residual r` is the residual we got when evaluating some element of
+        -- the record
+        simp at h₅ ; subst h₅
+        apply value_unknown (x := r)
+        case _ =>
+          simp [List.mem_map]
+          exists (a, .residual r)
+        case _ =>
+          have ⟨(a', x), h₆, h₇⟩ := mem_mapM_ok h₂ h₃
+          -- `x` is the record value which evaluated to `.residual r`
+          simp [Partial.bindAttr] at h₇
+          cases h₈ : Partial.evaluate x request entities
+          all_goals simp [h₈] at h₇
+          replace ⟨h₇, h₅⟩ := h₇
+          subst a' h₅
+          exact ih₁ (a, x) h₆ r h₈
+
+end Cedar.Thm.Partial.Evaluation.Record
