cedar-lean/Cedar/Thm/Utils.lean
@@ -36,17 +36,9 @@ theorem if_f_produces_pure_then_mapM_f_is_pure_map {α β} [Monad m] [LawfulMona
   case cons x xs h => simp [h]
 
 /--
-  A generic lemma about composing List.mapM with List.map. Not in Std AFAICT.
--/
-theorem mapM_map {α β γ} [Monad m] [LawfulMonad m] {f : α → β} {g : β → m γ} {xs : List α} :
-  List.mapM g (xs.map f) = xs.mapM fun x => g (f x)
-:= by
-  induction xs
-  case nil => simp
-  case cons x xs h => simp [h]
-
-/--
   A generic lemma about the behavior of List.mapM in the Option monad
+
+  The `mp` direction is a corollary of `mapM_eq_some` below, if we ever prove that
 -/
 theorem mapM_some_iff_f_some_on_all_elements {f : α → Option β} {xs : List α} :
   Option.isSome (xs.mapM f) ↔ ∀ x ∈ xs, Option.isSome (f x)
@@ -83,7 +75,29 @@ theorem mapM_some_iff_f_some_on_all_elements {f : α → Option β} {xs : List �
       sorry
 
 /--
-  Corollary of the above
+  Analogue of `mapM_some_iff_f_some_on_all_elements` for Map.mapMOnValues
+-/
+theorem mapMOnValues_some_iff_f_some_on_all_values [LT α] [DecidableLT α] {f : β → Option γ} {m : Map α β} :
+  Option.isSome (m.mapMOnValues f) ↔ ∀ v ∈ m.values, Option.isSome (f v)
+:= by
+  constructor
+  case mp =>
+    sorry
+  case mpr =>
+    sorry
+
+/--
+  A generic lemma about the behavior of List.mapM in the Option monad.
+-/
+theorem mapM_eq_some {f : α → Option β} {xs : List α} {ys : List β} {x : α} :
+  (xs.mapM f = some ys) → x ∈ xs → ∃ y ∈ ys, f x = some y
+:= by
+  rw [← List.mapM'_eq_mapM]
+  intro h₁ h₂
+  sorry
+
+/--
+  Corollary of `mapM_some_iff_f_some_on_all_elements`
 -/
 theorem mapM_none_iff_f_none_on_some_element {f : α → Option β} {xs : List α} :
   xs.mapM f = none ↔ ∃ x ∈ xs, f x = none
@@ -109,6 +123,48 @@ theorem mapM_none_iff_f_none_on_some_element {f : α → Option β} {xs : List �
     intro h₃
     rw [mapM_some_iff_f_some_on_all_elements] at h₃
     specialize h₃ x h₁
+    simp [h₂] at h₃
+
+/--
+  Analogue of `mapM_eq_some` for Map.mapMOnValues in the Option monad
+-/
+theorem mapMOnValues_eq_some [LT α] [DecidableLT α] {f : β → Option γ} {m₁ : Map α β} {m₂ : Map α γ} {k : α} {v : β} :
+  (m₁.mapMOnValues f = some m₂) → (k, v) ∈ m₁.kvs → ∃ v', (k, v') ∈ m₂.kvs ∧ f v = some v'
+:= by
+  intro h₁ h₂
+  sorry
+
+/--
+  Analogue of `mapM_none_iff_f_none_on_some_element` for Map.mapMOnValues
+
+  Corollary of `mapMOnValues_some_iff_f_some_on_all_values`
+-/
+theorem mapMOnValues_none_iff_f_none_on_some_value [LT α] [DecidableLT α] {f : β → Option γ} {m : Map α β} :
+  m.mapMOnValues f = none ↔ ∃ v ∈ m.values, f v = none
+:= by
+  -- As of this writing, this proof is nearly syntactically identical to the
+  -- proof of `mapM_none_iff_f_none_on_some_element`
+  constructor
+  case mp =>
+    intro h₁
+    by_contra h₂
+    replace h₂ := forall_not_of_not_exists h₂
+    simp only [not_and] at h₂
+    rw [← Option.not_isSome_iff_eq_none] at h₁
+    rw [mapMOnValues_some_iff_f_some_on_all_values] at h₁
+    apply h₁ ; clear h₁
+    intro v h₁
+    specialize h₂ v h₁
+    rw [← ne_eq] at h₂
+    rw [Option.ne_none_iff_isSome] at h₂
+    exact h₂
+  case mpr =>
+    intro h₁
+    replace ⟨v, h₁, h₂⟩ := h₁
+    rw [← Option.not_isSome_iff_eq_none]
+    intro h₃
+    rw [mapMOnValues_some_iff_f_some_on_all_values] at h₃
+    specialize h₃ v h₁
     simp [h₂] at h₃
 
 /--
@@ -158,17 +214,41 @@ theorem mapM_ok_iff_f_ok_on_all_elements {f : α → Except ε β} {xs : List α
             cases h₃
 
 /--
+  Corollary of the above
+-/
+theorem mapM_err_iff_f_err_on_some_element {f : α → Except ε β} {xs : List α} :
+  ¬ Except.isOk (xs.mapM f) ↔ ∃ x ∈ xs, ¬ Except.isOk (f x)
+:= by
+  sorry
+
+/--
   Another generic lemma about the behavior of List.mapM in the Option monad
 -/
-theorem mem_mapM_some {f : α → Option β} {xs : List α} {y : β} :
+theorem mem_mapM_some {f : α → Option β} {xs : List α} {ys : List β} {y : β} :
   xs.mapM f = some ys → y ∈ ys → ∃ x ∈ xs, f x = some y
+:= by
+  sorry
+
+/--
+  Analogue of `mem_mapM_some` for Map.mapMOnValues in the Option monad
+-/
+theorem mem_mapMOnValues_some [LT α] [DecidableLT α] {f : β → Option γ} {m₁ : Map α β} {m₂ : Map α γ} {k : α} {y : γ} :
+  m₁.mapMOnValues f = some m₂ → (k, y) ∈ m₂.kvs → ∃ v, (k, v) ∈ m₁.kvs ∧ f v = some y
 := by
   sorry
 
 /--
   Another generic lemma about the behavior of List.mapM in the Except monad
 -/
-theorem mem_mapM_ok {f : α → Except ε β} {xs : List α} {y : β} :
+theorem mem_mapM_ok {f : α → Except ε β} {xs : List α} {ys : List β} {y : β} :
   xs.mapM f = .ok ys → y ∈ ys → ∃ x ∈ xs, f x = .ok y
+:= by
+  sorry
+
+/--
+  Another generic lemma about the behavior of List.mapM in the Except monad
+-/
+theorem mem_mapM_err {f : α → Except ε β} {xs : List α} {e : ε} :
+  xs.mapM f = .error e ↔ ∃ x ∈ xs, f x = .error e
 := by
   sorry
